Update split_test2.dfy
wrote split and FindNextDelimiter functions, but cannot prove split function yet.

split_test2.dfy
@@ -1,4 +1,106 @@
-function method split(input:string, delimiter:char, index:int)
+function method FindNextDelimiter(input:string, delimiter:char, index :nat)
+    :(output:nat)
+    requires 0 <= index < |input|
+    requires delimiter in input[index..]
+    decreases |input|-index
+    ensures index <= output < |input|
+    ensures input[output] == delimiter
+    ensures delimiter !in input[index..output]
 {
+    if input[index] == delimiter then
+        index
+    else
+        FindNextDelimiter(input, delimiter, index+1)
+}
+
+function Join(s: seq<string>, d: char)
+    :(output: string)
+{
+    if |s| == 0 then
+        []
+    else
+        s[0] + [d] + Join(s[1..], d)
+}
+
+function split(s:string, d:char)
+    :(output:seq<string>)
+    // ensures forall o <- output :: d !in o
+    ensures 0 < |output|
+    // ensures Join(output, d) == s
+{
+    if d !in s then
+        [s]
+    else
+        var index := FindNextDelimiter(s,d,0);
+        [s[..index]]+split(s[index+1..],d)
+}
+
+lemma help_split(s:string,d:char)
+{
+    if s == ""
+    {
+        assert |split(s,d)| == 1;
+        assert multiset(s)[d]+1 == 1;
+
+    }
+    else if s[0] == d
+    {
+        assert multiset(s)[d]+1 >= 2;
+        assert |split(s,d)| >= 2;
+    }
+    // else if d in s
+    // {
+    //     assert multiset(s)[d]+1 == |split(s,d)|;
+    // }
+    else if d !in s
+    {
+        assert |split(s,d)| == multiset(s)[d]+1;
+    }
+}
+
+lemma tttt(s:string, d:char)
+    requires  multiset(s)[d] == 1;
+{
+    assert d in s;
+    var asdf := FindNextDelimiter(s, d, 0);
+
+    var a := s[..asdf];
+    var b := s[asdf + 1 ..];
+
+    assert d !in a;
+    assert s == a + [d] + b;
+    assert d !in b;
+
+
+    
+    // assert d !in b;
+
+
+}
+
+lemma test2(s:string, d:char, n:nat)
+    requires |split(s, d)| == n
+    requires n == 2
+    // ensures d !in s
+    ensures multiset(s)[d] == 1
+{
+    assert d in s;
+}
+
+method qwer(s:string, d:char)
+    requires d in s
+    // requires 0< |s| < 2
+    requires d == 'a'
+    requires s == "aa"
+
+{
+    // var s:= "abcs";
+    // var d:= 'a';
+    var h := multiset(s);
+    var j := h['a']+1;
+    // assert j == |split(s,d)|;
+    assert multiset("aa")['a']+1 == |split("aa",'a')|;
     
 }
+
+
